Save a proof for rwmutex with `rwmutexMaxReaders=-(1<<31)`;
really, the actual max readers is `(1<<31)-1`. One must write
`-(1<<31)` so it's representable as an int32. Here's the patch for
1.24.7 for posterity:

```
--- a/rwmutex.go
+++ b/rwmutex.go
@@ -44,7 +44,7 @@ type RWMutex struct {
        readerWait  atomic.Int32 // number of departing readers
 }

-const rwmutexMaxReaders = (1 << 30)
+const rwmutexMaxReaders = -(1<<31)

 // Happens-before relationships are indicated to the race detector via:
 // - Unlock  -> Lock:  readerSem
@@ -127,7 +127,7 @@ func (rw *RWMutex) RUnlock() {
 }

 func (rw *RWMutex) rUnlockSlow(r int32) {
-       if r+1 == 0 || r+1 == -rwmutexMaxReaders {
+       if r+1 == 0 || r+1 == rwmutexMaxReaders {
                race.Enable()
                fatal("sync: RUnlock of unlocked RWMutex")
        }
@@ -149,7 +149,7 @@ func (rw *RWMutex) Lock() {
        // First, resolve competition with other writers.
        rw.w.Lock()
        // Announce to readers there is a pending writer.
-       r := rw.readerCount.Add(-rwmutexMaxReaders) + rwmutexMaxReaders
+       r := rw.readerCount.Add(rwmutexMaxReaders) + rwmutexMaxReaders
        // Wait for active readers.
        if r != 0 && rw.readerWait.Add(r) != 0 {
                runtime_SemacquireRWMutex(&rw.writerSem, false, 0)
@@ -177,7 +177,7 @@ func (rw *RWMutex) TryLock() bool {
                }
                return false
        }
-       if !rw.readerCount.CompareAndSwap(0, -rwmutexMaxReaders) {
+       if !rw.readerCount.CompareAndSwap(0, rwmutexMaxReaders) {
                rw.w.Unlock()
                if race.Enabled {
                        race.Enable()
@@ -207,7 +207,7 @@ func (rw *RWMutex) Unlock() {

        // Announce to readers there is no active writer.
        r := rw.readerCount.Add(rwmutexMaxReaders)
-       if r >= rwmutexMaxReaders {
+       if r < 0 {
                race.Enable()
                fatal("sync: Unlock of unlocked RWMutex")
        }
```

new/code/sync.v
@@ -301,7 +301,7 @@ Definition RWMutex : go_type := structT [
 #[global] Typeclasses Opaque RWMutex.
 #[global] Opaque RWMutex.
 
-Definition rwmutexMaxReaders : Z := 1073741824.
+Definition rwmutexMaxReaders : Z := -2147483648.
 
 (* RLock locks rw for reading.
 
@@ -411,7 +411,7 @@ Definition RWMutex__rUnlockSlowⁱᵐᵖˡ : val :=
   λ: "rw" "r",
     exception_do (let: "rw" := (mem.alloc "rw") in
     let: "r" := (mem.alloc "r") in
-    (if: (((![#int32T] "r") + #(W32 1)) = #(W32 0)) || (((![#int32T] "r") + #(W32 1)) = #(W32 (- rwmutexMaxReaders)))
+    (if: (((![#int32T] "r") + #(W32 1)) = #(W32 0)) || (((![#int32T] "r") + #(W32 1)) = #(W32 rwmutexMaxReaders))
     then
       do:  ((func_call #race.Enable) #());;;
       do:  (let: "$a0" := #"sync: RUnlock of unlocked RWMutex"%go in
@@ -443,7 +443,7 @@ Definition RWMutex__Lockⁱᵐᵖˡ : val :=
     else do:  #());;;
     do:  ((method_call #(ptrT.id Mutex.id) #"Lock"%go (struct.field_ref #RWMutex #"w"%go (![#ptrT] "rw"))) #());;;
     let: "r" := (mem.alloc (type.zero_val #int32T)) in
-    let: "$r0" := ((let: "$a0" := #(W32 (- rwmutexMaxReaders)) in
+    let: "$r0" := ((let: "$a0" := #(W32 rwmutexMaxReaders) in
     (method_call #(ptrT.id atomic.Int32.id) #"Add"%go (struct.field_ref #RWMutex #"readerCount"%go (![#ptrT] "rw"))) "$a0") + #(W32 rwmutexMaxReaders)) in
     do:  ("r" <-[#int32T] "$r0");;;
     (if: ((![#int32T] "r") ≠ #(W32 0)) && ((let: "$a0" := (![#int32T] "r") in
@@ -488,7 +488,7 @@ Definition RWMutex__TryLockⁱᵐᵖˡ : val :=
       return: (#false)
     else do:  #());;;
     (if: (~ (let: "$a0" := #(W32 0) in
-    let: "$a1" := #(W32 (- rwmutexMaxReaders)) in
+    let: "$a1" := #(W32 rwmutexMaxReaders) in
     (method_call #(ptrT.id atomic.Int32.id) #"CompareAndSwap"%go (struct.field_ref #RWMutex #"readerCount"%go (![#ptrT] "rw"))) "$a0" "$a1"))
     then
       do:  ((method_call #(ptrT.id Mutex.id) #"Unlock"%go (struct.field_ref #RWMutex #"w"%go (![#ptrT] "rw"))) #());;;
@@ -530,7 +530,7 @@ Definition RWMutex__Unlockⁱᵐᵖˡ : val :=
     let: "$r0" := (let: "$a0" := #(W32 rwmutexMaxReaders) in
     (method_call #(ptrT.id atomic.Int32.id) #"Add"%go (struct.field_ref #RWMutex #"readerCount"%go (![#ptrT] "rw"))) "$a0") in
     do:  ("r" <-[#int32T] "$r0");;;
-    (if: int_geq (![#int32T] "r") #(W32 rwmutexMaxReaders)
+    (if: int_lt (![#int32T] "r") #(W32 0)
     then
       do:  ((func_call #race.Enable) #());;;
       do:  (let: "$a0" := #"sync: Unlock of unlocked RWMutex"%go in
